

6.2: Integration by Substitution

Example. Find the derivative of the following functions:

$$f(x) = \frac{(2x+1)^4}{4}$$
$$f'(x) = \frac{4(2x+1)^3}{4} \cdot 2 = \boxed{2(2x+1)^3}$$

$$g(x) = \frac{1}{x+3} = (x+3)^{-1}$$

$$g'(x) = -1(x+3)^{-2} \cdot 1 = \boxed{\frac{-1}{(x+3)^2}}$$

Let $u = g(x)$, where g is differentiable on an interval, and let f be continuous on the corresponding range of g . On that interval,

$$\int f'(g(x)) \cdot g'(x) dx = \int f(u) du$$

Procedure: Substitution Rule (Change of Variables)

1. Let $u = g(x)$, where $g(x)$ is part of the integrand, usually the “inside function” of a composite function $f(g(x))$.
2. Find $du = g'(x) dx$.
3. Use the substitution $u = g(x)$ and $du = g'(x) dx$ to convert the *entire* integral into one involving only u .
4. Find the resulting integral
5. Replace u by $g(x)$ to obtain the final solution as a function of x .

Example. Evaluate the following integrals:

$$\begin{aligned}\int \underline{2x}(x^2 + 3)^4 \underline{dx} &= \int u^4 du \\ u &= x^2 + 3 \\ du &= 2x dx \\ &= \frac{u^5}{5} + C \\ &= \boxed{\frac{1}{5} (x^2 + 3)^5 + C}\end{aligned}$$

$$\begin{aligned}\int (2x + 1)^3 dx &= \int u^3 \cdot \frac{1}{2} du \\ u &= 2x + 1 \\ du &= 2 dx \\ &\downarrow \\ \frac{1}{2} du &= dx \\ &= \frac{u^4}{4} \cdot \frac{1}{2} + C \\ &= \boxed{\frac{(2x + 1)^4}{8} + C}\end{aligned}$$

$$\int \underline{x^2} \sqrt{x^3+1} \underline{dx} = \int u^{1/2} \cdot \frac{1}{3} du$$

$$u = x^3 + 1$$

$$du = 3x^2 dx$$

$$\downarrow$$

$$\frac{1}{3} du = x^2 dx$$

$$= \frac{u^{3/2}}{3/2} \cdot \frac{1}{3} + C$$

$$= \boxed{\frac{2(x^3+1)^{3/2}}{9} + C}$$

$$\int \underline{t} \sqrt[4]{1-t^2} \underline{dt} = -\frac{1}{2} \int u^{1/2} du$$

$$u = 1 - t^2$$

$$du = -2t dt$$

$$\downarrow$$

$$-\frac{1}{2} du = t dt$$

$$= -\frac{1}{2} \frac{u^{3/2}}{3/2} + C$$

$$= \boxed{-\frac{1}{3}(1-t^2)^{3/2} + C}$$

$$\int \sqrt{4-t} dt = -\int u^{1/2} du$$

$$u = 4 - t$$

$$du = -dt$$

$$= -\frac{u^{3/2}}{3/2} + C$$

$$= \boxed{-\frac{2}{3}(4-t)^{3/2} + C}$$

$$\int (2-x)^6 dx = -\int u^6 dx$$

$$u = 2 - x$$

$$du = -dx$$

$$= -\frac{u^7}{7} + C$$

$$= \boxed{-\frac{(2-x)^7}{7} + C}$$

$$\int e^{-3x} dx = -\frac{1}{3} \int e^u du$$

$$\begin{aligned} u &= -3x \\ du &= -3 dx \\ &= -\frac{1}{3} e^u + C \\ &= \boxed{-\frac{1}{3} e^{-3x} + C} \end{aligned}$$

$$\int \frac{t}{3t^2+1} dt = \frac{1}{6} \int \frac{1}{u} du$$

$$\begin{aligned} u &= 3t^2+1 \\ du &= 6t dt \\ &= \frac{1}{6} \ln|u| + C \\ &= \boxed{\frac{1}{6} \ln(3t^2+1) + C} \end{aligned}$$

$$\int \frac{(\ln(x))^2}{2x} dx = \frac{1}{2} \int (\ln(x))^2 \cdot \frac{1}{x} dx$$

$$\begin{aligned} u &= \ln(x) \\ du &= \frac{1}{x} dx \end{aligned}$$

$$\begin{aligned} &= \frac{1}{2} \int u^2 du \\ &= \frac{1}{2} \frac{u^3}{3} + C \\ &= \boxed{\frac{1}{6} (\ln(x))^3 + C} \end{aligned}$$

$$\int u^3 (u^2+1)^{3/2} du = \int u^2 (u^2+1)^{3/2} u du$$

$$\begin{aligned} v &= u^2+1 \\ dv &= 2u du \\ \rightarrow v-1 &= u^2 \end{aligned}$$

$$\begin{aligned} &= \int (v-1) v^{3/2} dv \\ &= \int v^{5/2} - v^{3/2} dv \\ &= \frac{v^{7/2}}{7/2} - \frac{v^{5/2}}{5/2} + C \end{aligned}$$

$$= \boxed{\frac{2}{7} (u^2+1)^{7/2} - \frac{2}{5} (u^2+1)^{5/2} + C}$$